AP/DigitalRoot.lean
@@ -1,1 +1,3 @@
-import AP.DigitalRoot.Main
+import AP.DigitalRoot.Basic
+import AP.DigitalRoot.List
+import AP.DigitalRoot.Time
