AP/DigitalRoot/List.lean
@@ -1,0 +1,6 @@
+import AP.DigitalRoot.Basic
+
+namespace DigitalRoot
+
+def digRootList (b : ℕ) (xs : List ℕ) : ℕ :=
+  digRoot b xs.sum
