AP/DigitalRoot/Time.lean
@@ -1,0 +1,148 @@
+import AP.DigitalRoot.List
+
+section logic
+
+@[simp]
+theorem choose?_eq_some_iff {α : Type*} {p : α → Prop} {x}
+[hp : Decidable # ∃ x, p x] : choose? p = some x ↔ p x ∧
+haveI : Inhabited α := ⟨x⟩; Classical.epsilon p = x := by
+  have h₁ : Inhabited α := ⟨x⟩; simp [choose?]; constructor
+  · rintro ⟨h₂, rfl⟩; use h₂.choose_spec, choose_eq_epsilon h₂ |>.symm
+  · rintro ⟨h₂, h₃⟩; use ⟨_, h₂⟩; rwa [choose_eq_epsilon ⟨_, h₂⟩]
+
+theorem epsilon_eq_of_exiu {α : Type*} [ha : Inhabited α] {p : α → Prop} {x}
+(h₁ : p x) (h₂ : ∃! x, p x) : Classical.epsilon p = x := by
+  have hp : p = λ y => x = y
+  · ext y; obtain ⟨z, h₂, h₃⟩ := h₂
+    constructor <;> intro h₄
+    · rw [h₃ _ h₁, h₃ _ h₄]
+    · rwa [←h₄]
+  have h₃ := Classical.epsilon_spec h₂
+  dsimp at h₃; subst hp; simp at h₃; exact h₃.symm
+
+theorem epsilon_eq_of {α : Type*} [ha : Inhabited α] {p : α → Prop} {x}
+(h₁ : p x) (h₂ : ∀ y, p y → y = x) : Classical.epsilon p = x := by
+  apply epsilon_eq_of_exiu h₁; use x
+
+-- #check 0 #exit
+
+end logic
+
+section order
+
+variable {α : Type*} [ha₁ : DecidableEq α] [ha₂ : Fintype α]
+
+noncomputable
+def fintypeIdx (x : α) : ℕ :=
+  Finset.univ.toList.idxOf x
+
+@[simp]
+theorem fintypeIdx_eq_iff {x y : α} : fintypeIdx x = fintypeIdx y ↔ x = y := by
+  symm; constructor; rintro rfl; rfl; intro h; unfold fintypeIdx at h
+  rwa [List.idxOf_inj] at h <;> simp
+
+open Classical in noncomputable
+def fintypeToLinearOrder : LinearOrder α where
+  le a b := fintypeIdx a ≤ fintypeIdx b
+  le_refl a := by rfl
+  le_trans a b c h₁ h₂ := h₁.trans h₂
+  le_antisymm a b h₁ h₂ := by
+    have h₃ := le_antisymm h₁ h₂
+    simp at h₃; exact h₃
+  le_total a b := by apply le_total
+  toDecidableLE := by infer_instance
+
+-- #check 0 #exit
+
+end order
+
+namespace Map
+
+variable {α : Type*} [ha₁ : LinearOrder α] [ha₂ : Hashable α]
+variable {mp mp₁ mp₂ : Map α ℕ}
+
+def push (mp : Map α ℕ) (i : α) : Map α ℕ :=
+  mp.insert i # (mp.get? i).getD 0 + 1
+
+theorem get?_insert {i j x} :
+(mp.insert j x).get? i = if j = i then some x else mp.get? i := by
+  convert mp.1.get?_insert; simp; rfl
+
+theorem push_push_comm {i j} : (mp.push i).push j = (mp.push j).push i := by
+  ext; simp [push, get?_insert]; aesop
+
+-- #check 0 #exit
+
+end Map
+
+namespace DigitalRoot
+
+structure Time : Type where
+  hour : Fin 24
+  minute : Fin 60
+deriving Inhabited, DecidableEq, Fintype, Hashable
+
+def Time.toList (t : Time) : List ℕ :=
+  [t.hour, t.minute]
+
+@[simp]
+def timeSet : Set' Time := Set'.univ
+
+def digRootTime (b : ℕ) (t : Time) : ℕ :=
+  digRootList b t.toList
+
+open Classical in noncomputable
+def freqTimeDig (b : ℕ) : Option ℕ := choose? # λ d =>
+  let f d₁ := timeSet.count (digRootTime b · = d₁)
+  d ≤ b ∧ ∀ d', d' ≠ d → f d' < f d
+
+def freqTimeDigFn (b : ℕ) (mp : Map ℕ ℕ) (t : Time) : Map ℕ ℕ :=
+  mp.push # digRootTime b t
+
+theorem freqTimeDigFn_freqTimeDigFn_comm {b} {mp : Map ℕ ℕ} {t₁ t₂ : Time} :
+freqTimeDigFn b (freqTimeDigFn b mp t₁) t₂ = freqTimeDigFn b (freqTimeDigFn b mp t₂) t₁ :=
+  Map.push_push_comm
+
+def freqTimeDig' (b : ℕ) : Option ℕ := do
+  let res : Map ℕ ℕ := timeSet.fold (freqTimeDigFn b) ∅
+    freqTimeDigFn_freqTimeDigFn_comm
+  let xs := res.toList.mergeSort # λ a b => b.2 ≤ a.2
+  match xs with
+  | (d₁, c₁) :: (_, c₂) :: _ => do
+    guard # c₁ ≠ c₂
+    pure d₁
+  | _ => none
+
+-- variable {b} [hb : Base b]
+
+-- #check 0 #exit
+
+theorem freqTimeDig_eq_freqTimeDig' {b} : freqTimeDig b = freqTimeDig' b := by
+  have H := fintypeToLinearOrder (α := Time)
+  ext d
+  simp [freqTimeDig, freqTimeDig']
+  constructor
+  · rintro ⟨⟨h₁, h₂⟩, -⟩
+    rw [Set'.fold_eq_foldl_toList]
+    sorry
+  · intro h
+    split at h <;> simp at h
+    nm xs d₁ c₁ d₂ c₂ ys h₁
+    rcases h with ⟨h, rfl⟩
+    apply and_of
+    · constructor
+      · sorry
+      · intro d' h₂
+        sorry
+    rintro ⟨h₂, h₃⟩
+    apply epsilon_eq_of ⟨h₂, h₃⟩
+    rintro d₁' ⟨h₄, h₅⟩
+    by_contra! h₆
+    specialize h₃ _ h₆
+    specialize h₅ _ # ne_symm' h₆
+    linarith
+
+-- #check 0 #exit
+
+theorem freqTimeDig_10_eq_some_5 : freqTimeDig 10 = some 5 := by
+  rw [freqTimeDig_eq_freqTimeDig']; native_decide
